\documentclass{beamer}

 

\usepackage[utf8]{inputenc}

 

 

%Information to be included in the title page:

\title{Presentation}

\author{Shreekara Raghavan}

\institute{ee18btech11040}

\date{12 February 2020}

 

 

 

\begin{document}

 

\frame{\titlepage}

 

\begin{frame}

\frametitle{The Question}

The transfer function of the system Y(s)/U(s) whose state-space equations are given below:



\begin{bmatrix} x_1'(t)\\ x_2'(t) \end{bmatrix} = \begin{bmatrix}  1&2\\ 2&0 \end{bmatrix}\begin{bmatrix} x_1(t)\\ x_2(t) \end{bmatrix} + \begin{bmatrix} 1 \\ 2 \end{bmatrix}u(t)    ........(1)



y(t) = \begin{bmatrix} 1&0 \end{bmatrix}\begin{bmatrix} x_1(t)\\ x_2(t) \end{bmatrix}    ............(2)















(A) \(\frac{s + 2}{s^2 - 2s - 2}\)  (B) \(\frac{s - 2}{s^2 + s - 4}\) (C) \(\frac{s - 4}{s^2 + s - 4}\)  (D) \(\frac{s + 4}{s^2 - s - 4}\)



\end{frame}



\begin{frame}

\frametitle{Answer}

Consider equation 1, which can be written as

\centerline{X'(t) = AX(t) + BU(t)}

where

A = \begin{bmatrix}  1&2\\ 2&0 \end{bmatrix} and B = \begin{bmatrix} 1&0 \end{bmatrix}



Taking Laplace Transform on both sides





\centerline{sX(s) = AX(s) + BU(s)}

\centerline{X(s)(sI - A) = BU(s)}

\centerline{X(s) = (sI - A)^{-1} BU(s)}









\end{frame}

 

 

\begin{frame}

\frametitle{Answer Continued..}

From equation 2 we get

\centerline{Y(t) = CX(t)}

where C = \begin{bmatrix}1&0\end{bmatrix}

after taking Laplace transform becomes

\centerline{Y(s) = CX(s) }

The same equation can then be written as 

\centerline{Y(s) = C(sI - A)^{-1} BU(s)}





\end{frame}

  

\begin{frame}{Answer Continued....}



Thus our transfer function can be written as 

\centerline{H(s) = \(\frac{Y(s)}{U(s)}\) = C(sI - A)^{-1} B}

    

\end{frame}



\begin{frame}{Some Simplification}

H(s) = \begin{bmatrix}1&0\end{bmatrix}\begin{bmatrix}  s-1&-2\\ -2&s \end{bmatrix}^{-1}\begin{bmatrix} 1\\2 \end{bmatrix}





H(s) = \begin{bmatrix}1&0\end{bmatrix}\(\frac{\begin{bmatrix}  s&2\\ 2&s-1 \end{bmatrix}}{s^2 -s - 4}\)\begin{bmatrix} 1\\2 \end{bmatrix}



H(s) = \begin{bmatrix}1&0\end{bmatrix}\(\frac{\begin{bmatrix}  s+4\\ 2+2s-2 \end{bmatrix}}{s^2 -s - 4}\)



H(s) = \(\frac{s + 4}{s^2 - s - 4}\)

    

\end{frame}



\end{document}
